Eddy diffusion 
\begin{equationCode}{EddyDiffusionEvaluator}
\begin{split}
\eddy              &     = \eddy_0  \sqrt{\frac{\concAtm(\zmin)}{\concAtm(z)}} \\
\uu [cm^2\,s^{-1}] & \uu = [cm^2\,s^{-1}] \left(\frac{[cm^{-3}]}{[cm^{-3}]}\right)^{\frac{1}{2}} \\
\end{split}
\label{Titan:eddy_diff}
\end{equationCode}

The derivatives are:
\begin{equationCode}{EddyDiffusionEvaluator}
\begin{split}
\doverd{\eddy}{\conc_k} & = - \frac{\eddy}{2\concAtm(z)} \\
\uu \frac{[cm^2\,s^{-1}]}{[cm^{-3}]} & \uu = -\frac{[cm^2\,s^{-1}]}{[cm^{-3}]}
\end{split}
\label{Titan:eddy_diff_der_n}
\end{equationCode}
%
and
%
\begin{equationCode}{EddyDiffusionEvaluator}
\begin{split}
\doverd{\eddy}{T} & = 0 \\
\uu \frac{[cm^2\,s^{-1}]}{[K]} & \uu = [cm^2\,s^{-1}\,K^{-1}]
\end{split}
\label{Titan:eddy_diff_der_T}
\end{equationCode}
